coq/theories/coc.v
@@ -1,0 +1,160 @@
+From mathcomp Require Import ssreflect ssrbool eqtype ssrnat seq.
+From Coq Require Import ssrfun Program.
+Require Import AutosubstSsr ARS.
+
+Set Implicit Arguments.
+Unset Strict Implicit.
+Unset Printing Implicit Defensive.
+
+Module CoC.
+
+Definition context T := seq (option T).
+Definition cons_Some T (n : T) (Gamma : context T) : context T := 
+  Some n :: Gamma.
+Definition cons_None T (Gamma : context T) : context T := 
+  None :: Gamma.
+
+Notation "m :s Gamma" := (cons_Some m Gamma) (at level 30).
+Notation ":n Gamma" := (cons_None Gamma) (at level 30).
+
+Inductive has {T} `{Ids T} `{Subst T} : 
+  context T -> var -> T -> Prop :=
+| has_O m Gamma :
+  has (m :s Gamma) 0 m.[ren (+1)]
+| has_S Gamma v m n : 
+  has Gamma v m ->
+  has (n :s Gamma) (v.+1) m.[ren (+1)]
+| has_N Gamma v m : 
+  has Gamma v m ->
+  has (:n Gamma) (v.+1) m.[ren (+1)].
+
+Lemma has_x {T} `{Ids T} `{Subst T} (Gamma : context T) x A :
+  has Gamma x A ->
+  forall B,
+    has Gamma x B ->
+    A = B.
+Proof.
+  induction 1; intros.
+  inv H1; eauto.
+  inv H2; eauto.
+  apply IHhas in H7. rewrite H7; eauto.
+  inv H2; eauto.
+  apply IHhas in H5. rewrite H5; eauto.
+Qed.
+  
+Inductive term : Type :=
+| Var (x : var)
+| Sort (n : nat)
+| App  (s t : term)
+| Lam  (s : {bind term})
+| Prod (s : term) (t : {bind term}).
+
+Instance Ids_term : Ids term. derive. Defined.
+Instance Rename_term : Rename term. derive. Defined.
+Instance Subst_term : Subst term. derive. Defined.
+Instance substLemmas_term : SubstLemmas term. derive. Qed.
+
+Inductive value : term -> Prop :=
+| value_sort l   : value (Sort l)
+| value_var x    : value (Var x)
+| value_prod A B : value (Prod A B)
+| value_lam n    : value (Lam n).
+
+Inductive step : term -> term -> Prop :=
+| step_beta s t u :
+  u = s.[t/] -> step (App (Lam s) t) u
+| step_appL s1 s2 t :
+  step s1 s2 -> step (App s1 t) (App s2 t)
+| step_appR s t1 t2 :
+  step t1 t2 -> step (App s t1) (App s t2)
+| step_lam s1 s2 :
+  step s1 s2 -> step (Lam s1) (Lam s2)
+| step_prodL A1 A2 B :
+  step A1 A2 -> step (Prod A1 B) (Prod A2 B)
+| step_prodR A B1 B2 :
+  step B1 B2 -> step (Prod A B1) (Prod A B2).
+
+Inductive pstep : term -> term -> Prop :=
+| pstep_beta s1 s2 t1 t2 u :
+  u = s2.[t2/] ->
+  pstep s1 s2 -> pstep t1 t2 -> pstep (App (Lam s1) t1) u
+| pstep_var x : pstep (Var x) (Var x)
+| pstep_sort n : pstep (Sort n) (Sort n)
+| pstep_app s1 s2 t1 t2 :
+  pstep s1 s2 -> pstep t1 t2 -> pstep (App s1 t1) (App s2 t2)
+| pstep_lam s1 s2 :
+  pstep s1 s2 -> pstep (Lam s1) (Lam s2)
+| pstep_prod s1 s2 t1 t2 :
+  pstep s1 s2 -> pstep t1 t2 -> pstep (Prod s1 t1) (Prod s2 t2).
+
+Notation red := (star pstep).
+Notation "s === t" := (conv pstep s t) (at level 50).
+
+Lemma pstep_refl s : pstep s s.
+Proof.
+  induction s; constructor; eauto.
+Qed.
+
+Axiom pstep_ren : forall s s' xi, 
+  pstep s s' -> pstep s.[ren xi] s'.[ren xi].
+Axiom church_rosser : CR pstep.
+
+Reserved Notation "[ Gamma |- ]".
+Reserved Notation "[ Gamma |- s :- A ]".
+
+Inductive has_type : context term -> term -> term -> Prop :=
+| ty_var Gamma x A :
+  has Gamma x A ->
+  [ Gamma |- Var x :- A ]
+| ty_sort Gamma n  :
+  [ Gamma |- Sort n :- Sort n.+1 ]
+| ty_prod Gamma A B n :
+  [ Gamma |- A :- Sort n ] ->
+  [ A :s Gamma |- B :- Sort n ] ->
+  [ Gamma |- Prod A B :- Sort n ]
+| ty_lam Gamma A B s n :
+  [ Gamma |- Prod A B :- Sort n ] ->
+  [ A :s Gamma |- s :- B ] ->
+  [ Gamma |- Lam s :- Prod A B ]
+| ty_app Gamma A B s t :
+  [ Gamma |- s :- Prod A B ] ->
+  [ Gamma |- t :- A ] ->
+  [ Gamma |- App s t :- B.[t/] ]
+| ty_conv Gamma A B s :
+  A === B ->
+  [ Gamma |- s :- A ] ->
+  [ Gamma |- s :- B ]
+where "[ Gamma |- s :- A ]" := (has_type Gamma s A).
+
+Inductive context_ok : context term -> Prop :=
+| ctx_nil :
+  [ nil |- ]
+| ctx_ncons Gamma A n :
+  [ Gamma |- A :- Sort n ] ->
+  [ Gamma |- ] ->
+  [ A :s Gamma |- ]
+where "[ Gamma |- ]" := (context_ok Gamma).
+
+Notation "[ Gamma |- s ]" := (exists n, [ Gamma |- s :- Sort n ]).
+
+Axiom weakening : 
+  forall Gamma s A B,
+  [ Gamma |- s :- A ] -> [ B :: Gamma |- s.[ren (+1)] :- A.[ren (+1)] ].
+
+Axiom preservation :
+  forall Gamma s A,
+  [ Gamma |- ] -> 
+  [ Gamma |- s :- A ] ->
+  forall t, pstep s t -> [ Gamma |- t :- A ].
+
+Axiom progress :
+  forall s A,
+  [ nil |- s :- A ] -> value s \/ exists s', step s s'.
+
+Axiom strong_norm :
+  forall Gamma s A,
+  [ Gamma |- ] ->
+  [ Gamma |- s :- A ] ->
+  exists v, value v /\ s === v.
+
+End CoC.
